checkpoint before renaming files.
git-svn-id: https://webdav.seas.upenn.edu/svn/sol/vol@3211 eef5ea85-cc2e-0410-bd84-0fae1f012da8

src/Interpreter/main.ml
@@ -1,7 +1,6 @@
 open Opsem
 open Dopsem
 open Ssa_interpreter
-open Ssa_dynamic
 open Printf
 open Llvm
 open Llvm_executionengine
