src/ssa/ssa_analysis.v
@@ -837,6 +837,898 @@ End Kildall.
 
 End Dataflow_Solver_Var_Top.
 
+(**********************************)
+(* Dom and Reaching analysis *)
+
+Require Import ssa_def.
+Require Import ssa_lib.
+Import LLVMsyntax.
+Import LLVMlib.
+
+Definition successors_terminator (tmn: terminator) : ls :=
+match tmn with
+| insn_return _ _ _ => nil
+| insn_return_void _ => nil
+| insn_br _ _ l1 l2 => l1::l2::nil
+| insn_br_uncond _ l1 => l1::nil
+| insn_unreachable _ => nil
+end.
+
+Fixpoint successors_blocks (bs: blocks) : ATree.t ls :=
+match bs with
+| nil => ATree.empty ls
+| block_intro l0 _ _ tmn :: bs' => 
+    ATree.set l0 (successors_terminator tmn) (successors_blocks bs')
+end.
+
+Fixpoint successors (f: fdef) : ATree.t ls :=
+let '(fdef_intro _ bs) := f in
+successors_blocks bs.
+
+Definition transfer (bound: set atom) (lbl: l) (before: Dominators.t bound) :=
+  Dominators.add _ before lbl.
+
+(** The static analysis itself is then an instantiation of Kildall's
+  generic solver for forward dataflow inequations. [analyze f]
+  returns a mapping from program points to mappings of pseudo-registers
+  to approximations.  It can fail to reach a fixpoint in a reasonable
+  number of iterations, in which case [None] is returned. *)
+
+Module DomDS := Dataflow_Solver_Var_Top(AtomNodeSet).
+
+Fixpoint bound_blocks (bs: blocks) : set atom :=
+match bs with
+| nil => empty_set _
+| block_intro l0 _ _ tmn :: bs' => l0::(bound_blocks bs')
+end.
+
+Definition bound_fdef (f: fdef) : set atom :=
+let '(fdef_intro _ bs) := f in
+bound_blocks bs.
+
+Lemma entry_dom : forall (bs:list block), 
+  {oresult : option (l * Dominators.BoundedSet (bound_blocks bs)) &
+     match oresult with
+     | None => bs = nil
+     | Some (le, Dominators.mkBoundedSet (l1::nil) _) => le = l1
+     | _ => False
+     end
+  }.
+Proof.
+  intros.
+  destruct bs; simpl in *.
+    exists None. auto.
+
+    destruct b.
+    assert (incl [l0] (l0 :: bound_blocks bs)) as J.
+      simpl_env.
+      apply incl_appl; auto using incl_refl.
+    exists (Some (l0, Dominators.mkBoundedSet _ [l0] J)).  
+    simpl. auto.
+Defined.
+
+Definition dom_analyze (f: fdef) : AMap.t (Dominators.t (bound_fdef f)) :=
+  let '(fdef_intro _ bs) := f in
+  let bound := bound_blocks bs in
+  let top := Dominators.top bound in
+  match entry_dom bs with
+  | (existT (Some (le, start)) _) =>
+      match DomDS.fixpoint bound (successors_blocks bs) (transfer bound) 
+        ((le, start) :: nil) with
+      | None => (AMap.set le start (AMap.init top))
+      | Some res => res
+      end
+  | (existT None _) => AMap.init top
+  end.
+
+(*
+Program Definition dom_analyze (f: fdef): AMap.t (Dominators.t (bound_fdef f)) :=
+  let bound := bound_fdef f in
+  let top := Dominators.top bound in
+  match getEntryBlock f with
+  | Some (block_intro le _ _ _) =>
+      match DomDS.fixpoint bound (successors f) (transfer bound) 
+        ((le, Dominators.mkBoundedSet _ [le] _) :: nil) with
+      | None => AMap.init top
+      | Some res => res
+      end
+  | None => AMap.init top
+  end.
+Next Obligation.
+  destruct f. 
+  destruct b; simpl in *; inv Heq_anonymous. 
+    simpl_env.
+    apply incl_appl; auto using incl_refl.
+Qed.
+*)
+
+Definition blockDominates (f: fdef) (b1 b2: block) : Prop :=
+let '(block_intro l1 _ _ _) := b1 in
+let '(block_intro l2 _ _ _) := b2 in
+let 'dt := dom_analyze f in
+let '(Dominators.mkBoundedSet els _) := AMap.get l2 dt in
+set_In l1 els.
+
+Definition blockStrictDominates (f: fdef) (b1 b2: block) : Prop :=
+let '(block_intro l1 _ _ _) := b1 in
+let '(block_intro l2 _ _ _) := b2 in
+let 'dt := dom_analyze f in
+let '(Dominators.mkBoundedSet els _) := AMap.get l2 dt in
+l1 <> l2 /\ set_In l1 els.
+
+Definition insnDominates (id1:id) (i2:insn) (b:block) : Prop :=
+match b with 
+| (block_intro l5 ps cs tmn) =>
+  match i2 with
+  | insn_terminator tmn2 =>
+      ((exists cs1, exists c1, exists cs2, 
+         cs = cs1++c1::cs2 /\ getCmdID c1 = Some id1) \/ 
+       (exists ps1, exists p1, exists ps2, 
+         ps = ps1++p1::ps2 /\ getPhiNodeID p1 = id1)
+       ) /\ tmn2 = tmn
+  | insn_cmd c2 =>
+      (exists ps1, exists p1, exists ps2, 
+         ps = ps1++p1::ps2 /\ getPhiNodeID p1 = id1) \/
+      (exists cs1, exists c1, exists cs2, exists cs3,
+         cs = cs1++c1::cs2 ++ c2 :: cs3 /\ getCmdID c1 = Some id1)
+  | _ => False
+  end
+end.
+
+Module ReachDS := Dataflow_Solver(LBoolean)(AtomNodeSet).
+
+Definition reachable_aux (f: fdef) : option (AMap.t bool) :=
+  match getEntryBlock f with
+  | Some (block_intro le _ _ _) =>
+     ReachDS.fixpoint (successors f) (fun pc r => r) ((le, true) :: nil)
+  | None => None
+  end.
+
+Definition reachable (f: fdef) : AMap.t bool :=
+  match reachable_aux f with  
+  | None => AMap.init true
+  | Some rs => rs
+  end.
+
+Definition isReachableFromEntry (f:fdef) (b1:block) : Prop :=
+let '(block_intro l1 _ _ _) := b1 in
+AMap.get l1 (reachable f).
+ 
+(********************************************)
+(** * Correctness of analysis *)
+
+Axiom atomset_eq__proof_irr2 : forall (* proof irrelevence *)
+  max
+  (contents' : ListSet.set atom)
+  (inbound' : incl contents' max)
+  a
+  (Heqdefs' : {|
+             DomDS.L.bs_contents := contents';
+             DomDS.L.bs_bound := inbound' |} = a),
+  contents' = Dominators.bs_contents max a.
+
+Lemma atomset_eq__proof_irr1 : forall
+  (bs : blocks)
+  (l' : l)
+  (t : AMap.t (DomDS.dt (bound_blocks bs)))
+  (contents' : ListSet.set atom)
+  (inbound' : incl contents' (bound_blocks bs))
+  (Heqdefs' : {|
+             DomDS.L.bs_contents := contents';
+             DomDS.L.bs_bound := inbound' |} = t !! l')
+  (bs_contents : ListSet.set atom)
+  (bs_bound0 : incl bs_contents (bound_blocks bs))
+  (HeqR2 : {|
+          DomDS.L.bs_contents := bs_contents;
+          DomDS.L.bs_bound := bs_bound0 |} = t !! l'),
+  contents' = bs_contents.
+Proof. 
+  intros.  
+  apply atomset_eq__proof_irr2 in Heqdefs'; subst.
+  apply atomset_eq__proof_irr2 in HeqR2; subst.
+  auto.
+Qed.
+
+Lemma reachable_entrypoint:
+  forall (f:fdef) l0 ps cs tmn, 
+    LLVMlib.getEntryBlock f = Some (block_intro l0 ps cs tmn) ->
+    (reachable f)!!l0 = true.
+Proof.
+  intros f l0 ps cs tmn Hentry. unfold reachable.
+  caseEq (reachable_aux f).
+    unfold reachable_aux; intros reach A.
+    rewrite Hentry in A.
+    assert (LBoolean.ge reach!!l0 true).
+      eapply ReachDS.fixpoint_entry. eexact A. auto with coqlib.
+    unfold LBoolean.ge in H. tauto.
+
+    intros. apply AMap.gi.
+Qed.
+
+Require Import ssa_props.
+
+Lemma successors_terminator__successors_blocks : forall
+  (bs : blocks)
+  (l0 : l)
+  (cs : phinodes)
+  (ps : cmds)
+  (tmn : terminator)
+  (l1 : l)
+  (HuniqF : uniqBlocks bs)
+  (HbInF : InBlocksB (block_intro l0 cs ps tmn) bs)
+  (Hin : In l1 (successors_terminator tmn)),
+  successors_terminator tmn = (successors_blocks bs) !!! l0.
+Proof.
+  intros.
+  induction bs.
+    inversion HbInF.
+  
+    assert (J:=HuniqF).
+    simpl_env in J.
+    apply uniqBlocks_inv in J.
+    destruct J as [J1 J2]. 
+    simpl in *.
+    apply orb_prop in HbInF.
+    destruct a.
+    destruct HbInF as [HbInF | HbInF].
+      unfold blockEqB in HbInF.
+      apply sumbool2bool_true in HbInF. inv HbInF.
+      unfold successors_list.
+      rewrite ATree.gss. auto.
+  
+      apply IHbs in J2; auto.
+      unfold successors_list in *.
+      destruct HuniqF as [J _].
+      inv J.
+      rewrite ATree.gso; auto.
+        clear - HbInF H1. 
+        eapply InBlocksB__NotIn; eauto.
+Qed.
+
+Lemma successors_predOfBlock : forall f l1 ps1 cs1 tmn1 l0 ps0 cs0 tmn0,
+  uniqFdef f ->
+  blockInFdefB (block_intro l1 ps1 cs1 tmn1) f = true ->
+  In l0 (successors_terminator tmn1) ->
+  In l1 (predOfBlock (block_intro l0 ps0 cs0 tmn0) (genBlockUseDef_fdef f)).
+Proof.
+  unfold predOfBlock.
+  destruct f. destruct f. intros.
+  destruct H as [H _].
+  generalize dependent l1.
+  generalize dependent ps1.
+  generalize dependent cs1.
+  generalize dependent tmn1.
+  generalize dependent l0.
+  generalize dependent ps0.
+  generalize dependent cs0.
+  generalize dependent tmn0.
+  induction b; intros; simpl in *.
+    inversion H0.
+
+    assert (G:=H). simpl_env in G.
+    apply uniqBlocks_inv in G.
+    destruct G as [G1 G2].
+    destruct a0. simpl.
+    apply orb_prop in H0.
+    destruct H0 as [H0 | H0].
+      apply blockEqB_inv in H0.
+      inv H0.
+      destruct t0; auto.
+        apply IHb with (ps1:=p)(cs1:=c)(tmn1:=insn_return i0 t0 v0); auto.
+        apply IHb with (ps1:=p)(cs1:=c)(tmn1:=insn_return_void i0); auto.
+
+        simpl in H1.
+        destruct H1 as [H1 | [H1 | H1]]; subst.
+          assert (J:=@lookupAL_update_udb_eq (update_udb nil l2 l3) l2 l0).
+          destruct J as [ls0 [J1 J2]].
+          apply lookupAL_genBlockUseDef_blocks_spec with (bs:=b) in J1; auto.
+          destruct J1 as [ls1 [J1 J3]].
+          rewrite J1. apply J3; auto.
+
+          assert (J:=@lookupAL_update_udb_eq nil l2 l0).
+          destruct J as [ls0 [J J0]].
+          apply lookupAL_update_udb_spec with (l1:=l2)(l2:=l1) in J; auto.
+          destruct J as [ls1 [J J1]].
+          apply lookupAL_genBlockUseDef_blocks_spec with (bs:=b) in J; auto.
+          destruct J as [ls2 [J J2]].
+          rewrite J. apply J2. apply J1. auto.
+
+          inversion H1.
+        simpl in H1.
+        destruct H1 as [H1 | H1]; subst.
+          assert (J:=@lookupAL_update_udb_eq nil l2 l0).
+          destruct J as [ls0 [J J0]].
+          apply lookupAL_genBlockUseDef_blocks_spec with (bs:=b) in J; auto.
+          destruct J as [ls2 [J J2]].
+          rewrite J. apply J2. auto.
+
+          inversion H1.
+
+        apply IHb with (ps1:=p)(cs1:=c)(tmn1:=insn_unreachable i0); auto.
+
+      eapply IHb in H1; eauto.
+        remember (lookupAL (list l) (genBlockUseDef_blocks b nil) l0) as R.
+        destruct R; try solve [inversion H1].
+        destruct H as [J1 J2].
+        simpl in J1.
+        inv J1.
+        apply InBlocksB_In in H0.
+        destruct (eq_atom_dec l1 l2); subst.
+          contradict H0; auto.
+
+          clear - HeqR H1.
+          simpl.
+          assert (usedef_block_inc nil 
+            (match t0 with
+             | insn_return _ _ _ => nil
+             | insn_return_void _ => nil
+             | insn_br _ _ l4 l5 => update_udb (update_udb nil l2 l5) l2 l4
+             | insn_br_uncond _ l4 => update_udb nil l2 l4
+             | insn_unreachable _ => nil
+             end)) as J.
+            intros x A J. inversion J.
+          apply genBlockUseDef_blocks_inc with (bs:=b) in J.
+          symmetry in HeqR.
+          apply J in HeqR.
+          destruct HeqR as [l4 [J1 J2]].
+          rewrite J1. apply J2 in H1; auto.
+Qed.
+
+Lemma reachable_successors:
+  forall f l0 cs ps tmn l1,
+  uniqFdef f ->
+  blockInFdefB (block_intro l0 cs ps tmn) f ->
+  In l1 (successors_terminator tmn) ->
+  (reachable f)!!l0 = true ->
+  (reachable f)!!l1 = true.
+Proof.
+  intros f l0 cs ps tmn l1 HuniqF HbInF Hin.
+  unfold reachable.
+  caseEq (reachable_aux f).
+    unfold reachable_aux. intro reach; intros.
+    remember (LLVMlib.getEntryBlock f) as R.
+    destruct R; inv H.
+    destruct b as [le ? ? ?].
+    assert (LBoolean.ge reach!!l1 reach!!l0) as J.
+      change (reach!!l0) with ((fun pc r => r) l0 (reach!!l0)).
+      eapply ReachDS.fixpoint_solution; eauto.
+        destruct f as [[?] bs]. simpl in *.
+        clear - HuniqF HbInF Hin. destruct HuniqF.
+        assert ((successors_terminator tmn) = (successors_blocks bs) !!! l0) 
+          as EQ.
+          eapply successors_terminator__successors_blocks; eauto.
+        rewrite <- EQ; auto.            
+    elim J; intro. congruence. auto.
+
+  intros. apply AMap.gi.
+Qed.
+
+Ltac tinv H := try solve [inv H].
+Import AtomSet.
+
+Lemma dom_entrypoint : forall f l0 ps cs tmn
+  (Hentry : LLVMlib.getEntryBlock f = Some (block_intro l0 ps cs tmn)),
+  incl (Dominators.bs_contents (bound_fdef f) ((dom_analyze f) !! l0)) [l0].
+Proof.
+  intros.
+  unfold dom_analyze.
+  destruct f.
+  remember (entry_dom b) as R.
+  destruct R as [R Hp].
+  destruct R as [[le start] | ].
+  Case "entry is good". 
+    remember (DomDS.fixpoint (bound_blocks b) (successors_blocks b)
+                (transfer (bound_blocks b)) ((le, start) :: nil)) as R1.
+    destruct start.
+    destruct bs_contents; tinv Hp.
+    destruct bs_contents; tinv Hp.
+    subst le. 
+    destruct b; try solve [inversion HeqR].
+    destruct b. simpl in HeqR. inversion HeqR. subst a.
+    simpl in Hentry. inversion Hentry. subst l0 p c t.
+    clear HeqR Hentry.    
+    destruct R1; subst.
+    SCase "analysis is done".
+      symmetry in HeqR1.
+      apply DomDS.fixpoint_entry with (n:=l1)(v:={|
+                DomDS.L.bs_contents := l1 :: nil;
+                DomDS.L.bs_bound := bs_bound |}) in HeqR1; simpl; eauto.
+      unfold DomDS.L.ge in HeqR1.
+      unfold DomDS.L.eq, DomDS.L.top, DomDS.L.bot, DomDS.L.sub in HeqR1.
+      simpl in *.
+
+      remember (t !! l1) as R.
+      destruct R.
+      erewrite <- atomset_eq__proof_irr2; eauto.
+      destruct HeqR1 as [HeqR1 | [ HeqR1 | HeqR1 ]]; auto.
+      SSCase "1".       
+        apply set_eq_empty_inv in HeqR1. subst.
+        intros x J. inversion J.
+      SSCase "2".   
+        eapply incl_set_eq_right; eauto using set_eq_sym.
+    
+    SCase "analysis fails".
+      simpl.      
+      rewrite AMap.gss. simpl.
+      apply incl_refl.
+
+  Case "entry is wrong". 
+    subst. inversion Hentry.
+Qed.
+
+(***************************)
+(* domination prop *)
+
+Fixpoint cmds_dominates_cmd (cs:cmds) (id0:id) : list atom :=
+match cs with
+| nil => nil
+| c1::cs' => 
+    let ctx := cmds_dominates_cmd cs' id0 in
+    if eq_atom_dec (getCmdLoc c1) id0 then nil
+    else
+      match getCmdID c1 with
+      | Some id1 => id1::ctx
+      | None => ctx
+      end
+end.
+
+Lemma NoDup__In_cmds_dominates_cmd : forall cs1 c cs2 id1,
+  NoDup (getCmdsLocs (cs1 ++ c :: cs2)) ->
+  In id1 (getCmdsIDs cs1) ->
+  In id1 (cmds_dominates_cmd (cs1 ++ c :: cs2) (getCmdLoc c)).
+Proof.
+  induction cs1; intros; simpl in *.
+    inversion H0.
+
+    inv H.
+    destruct (eq_atom_dec (getCmdLoc a) (getCmdLoc c)).
+      assert (False) as F.
+        apply H3. 
+        rewrite e.
+        rewrite getCmdsLocs_app. simpl.
+        apply in_or_app. right. simpl. auto.
+      inversion F.
+
+      destruct (getCmdID a); auto.
+      simpl in *. destruct H0 as [H0 | H0]; auto.
+Qed.   
+
+Definition inscope_of_block (f:fdef) (l1:l) (opt_ctx:option (list atom)) (lbl:l)
+  :=
+  match opt_ctx with
+  | Some ctx =>
+     match lookupBlockViaLabelFromFdef f lbl with
+     | None => None
+     | Some b => 
+         if eq_atom_dec lbl l1 then Some ctx
+         else Some (getBlockIDs b ++ ctx)
+     end
+  | None => None
+  end.
+
+Definition inscope_of_cmd (f:fdef) (b1:block) (c:cmd) : option (list atom) :=
+let id0 := getCmdLoc c in
+let '(block_intro l1 ps cs _) := b1 in
+let '(fdef_intro (fheader_intro _ _ _ la _) _) := f in
+let 'dt := dom_analyze f in
+let '(Dominators.mkBoundedSet els _) := AMap.get l1 dt in
+fold_left (inscope_of_block f l1) els
+  (Some (getPhiNodesIDs ps ++ cmds_dominates_cmd cs id0 ++ getArgsIDs la))
+.
+
+Definition inscope_of_tmn (f:fdef) (b1:block) (tmn:terminator) 
+  : option (list atom) :=
+let '(block_intro l1 ps cs _) := b1 in
+let '(fdef_intro (fheader_intro _ _ _ la _) _) := f in
+let 'dt := dom_analyze f in
+let '(Dominators.mkBoundedSet els _) := AMap.get l1 dt in
+fold_left (inscope_of_block f l1) els
+  (Some (getPhiNodesIDs ps ++ getCmdsIDs cs ++ getArgsIDs la))
+.
+
+Definition defs_dominate (f:fdef) (curb incomingb:block) (i:insn) 
+  : option (list atom) :=
+match i with
+| insn_phinode p => 
+    let '(block_intro _ _ _ tmn) := incomingb in
+    inscope_of_tmn f incomingb tmn
+| insn_cmd c => inscope_of_cmd f curb c
+| insn_terminator tmn => inscope_of_tmn f curb tmn
+end.
+
+Lemma getCmdsIDs__cmds_dominates_cmd : forall cs2' c',
+  ~ In (getCmdLoc c') (LLVMlib.getCmdsLocs cs2') ->
+  set_eq _ (getCmdsIDs (cs2' ++ [c']))
+  (cmds_dominates_cmd (cs2' ++ [c']) (getCmdLoc c') ++ 
+    match getCmdID c' with
+    | Some id1 => [id1]
+    | None => nil
+    end).   
+Proof.
+  induction cs2'; intros c' Hnotin.
+    simpl in *.
+    destruct (eq_atom_dec (getCmdLoc c') (getCmdLoc c')) as [_ | n];
+      try solve [contradict n; auto].
+      remember (getCmdID c') as R.
+      destruct R; simpl_env; apply set_eq_refl.
+
+    simpl in *.
+    assert (~ In (getCmdLoc c') (getCmdsLocs cs2')) as J.
+      auto.
+    apply IHcs2' in J.
+    remember (getCmdID a) as R1.
+    remember (getCmdID c') as R2.
+    destruct (eq_atom_dec (getCmdLoc a) (getCmdLoc c')); 
+      try solve [contradict e; auto].
+    destruct R1; auto.
+      simpl_env.
+      apply set_eq_app; auto using set_eq_refl.
+Qed.      
+
+Definition opt_set_eq (ops1 ops2:option (list atom)) : Prop :=
+match (ops1, ops2) with
+| (None, None) => True
+| (Some s1, Some s2) => set_eq _ s1 s2
+| _ => False
+end.
+
+Lemma inscope_of_block__opt_set_eq : forall f l1 l' opr1 opr2,
+  opt_set_eq opr1 opr2 ->
+  opt_set_eq (inscope_of_block f l1 opr1 l') (inscope_of_block f l1 opr2 l').
+Proof.
+  unfold inscope_of_block.
+  intros.
+  destruct (lookupBlockViaLabelFromFdef f l').
+    destruct (eq_atom_dec l' l1); subst.
+      destruct opr1.
+        destruct opr2; try solve [inversion H | auto].
+        destruct opr2; try solve [inversion H | auto].
+      unfold opt_set_eq in *.
+      destruct opr1.
+        destruct opr2; try solve [inversion H ].
+          apply set_eq_app; auto using set_eq_refl.
+        destruct opr2; try solve [inversion H | auto ].
+    unfold opt_set_eq in *.
+    destruct opr1.
+      destruct opr2; try solve [inversion H | auto].
+      destruct opr2; try solve [inversion H | auto].
+Qed.
+ 
+Lemma fold_left__opt_set_eq_aux : forall ls0 opr1 opr2 f l1,
+  opt_set_eq opr1 opr2 ->
+  opt_set_eq (fold_left (inscope_of_block f l1) ls0 opr1) 
+           (fold_left (inscope_of_block f l1) ls0 opr2).
+Proof.
+  induction ls0; intros opr1 opr2 f l1 Heq; simpl in *; auto.
+    apply IHls0.
+      apply inscope_of_block__opt_set_eq; auto.
+Qed.
+
+Lemma fold_left__opt_set_eq : forall (ls0:list atom) f l1 init1 init2 r1,
+  set_eq _ init1 init2 ->  
+  fold_left (inscope_of_block f l1) ls0 (Some init1) = Some r1 ->
+  exists r2, fold_left (inscope_of_block f l1) ls0 (Some init2) = Some r2 /\ 
+    set_eq _ r1 r2.
+Proof.
+  intros.
+  assert (opt_set_eq (Some init1) (Some init2)) as EQ. unfold opt_set_eq. auto.
+  apply fold_left__opt_set_eq_aux with (ls0:=ls0)(f:=f)(l1:=l1) in EQ.
+  remember (fold_left (inscope_of_block f l1) ls0 (ret init2)) as R. 
+  unfold opt_set_eq in EQ.    
+  rewrite H0 in EQ.
+  destruct R; try solve [inversion EQ].
+  exists l0. auto.
+Qed.
+ 
+Lemma inscope_of_block__opt_union : forall f l1 l' init1 init2 r1,
+  inscope_of_block f l1 (Some init1) l' = Some r1 ->
+  exists r2, inscope_of_block f l1 (Some (init1++init2)) l' = Some r2 /\
+    set_eq _ (r1++init2) r2.
+Proof.
+  intros.
+  unfold inscope_of_block in *.
+  destruct (lookupBlockViaLabelFromFdef f l').
+    destruct (eq_atom_dec l' l1); subst; inv H.
+      exists (r1++init2). auto using set_eq_refl.
+      exists (getBlockIDs b ++ init1 ++ init2). 
+        simpl_env. auto using set_eq_refl.
+    inversion H.
+Qed.
+
+Lemma fold_left__none : forall (ls0:list atom) f l1,
+  fold_left (inscope_of_block f l1) ls0 None = None.
+Proof.
+  induction ls0; intros f l1; simpl in *; auto.
+Qed.
+
+Lemma fold_left__opt_union : forall (ls0:list atom) f l1 init1 init2 r1,
+  fold_left (inscope_of_block f l1) ls0 (Some init1) = Some r1 ->
+  exists r2, 
+    fold_left (inscope_of_block f l1) ls0 (Some (init1++init2)) = Some r2 
+      /\ set_eq _ (r1++init2) r2.
+Proof.
+  induction ls0; intros f l1 init1 init2 r1 H; simpl in *; auto.
+    inv H. exists (r1 ++ init2). split; auto using set_eq_refl.
+
+    destruct (lookupBlockViaLabelFromFdef f a).
+      destruct (eq_atom_dec a l1); subst; auto.
+        apply IHls0 with (init2:=init2) in H; auto.
+          simpl_env in H. auto.
+      rewrite fold_left__none in H. inversion H.
+Qed.
+
+Lemma inscope_of_cmd_tmn : forall f l2 ps2 cs2' c' tmn' ids1,
+~ In (getCmdLoc c') (getCmdsLocs cs2') ->
+Some ids1 = inscope_of_cmd f (block_intro l2 ps2 (cs2'++[c']) tmn') c' ->
+exists ids2, 
+  Some ids2 = inscope_of_tmn f (block_intro l2 ps2 (cs2'++[c']) tmn') tmn' /\
+  match getCmdID c' with
+  | Some id1 => set_eq _ (id1::ids1) ids2
+  | None => set_eq _ ids1 ids2
+  end.
+Proof.
+  intros f l2 ps2 cs2' c' tmn' ids1 Hnotin Hinscope.
+  unfold inscope_of_cmd in Hinscope.
+  unfold inscope_of_tmn.
+  destruct f as [[? ? ? la va] bs].
+  remember ((dom_analyze (fdef_intro (fheader_intro f t i0 la va) bs)) !! l2) as R.
+  destruct R as [R_contents R_bound]. simpl in *.
+  apply getCmdsIDs__cmds_dominates_cmd in Hnotin.
+  symmetry in Hinscope.
+  remember (getCmdID c') as R.
+  destruct R.
+    apply fold_left__opt_union with (init2:=[i1]) in Hinscope.
+    destruct Hinscope as [r2 [Hinscope Heq]].
+    apply fold_left__opt_set_eq with (init2:=((getPhiNodesIDs ps2) ++
+      ((getCmdsIDs (cs2' ++ [c'])) ++ (getArgsIDs la)))) in Hinscope.
+      destruct Hinscope as [r3 [Hinscope Heq']].
+      exists r3.     
+      split; auto.
+        simpl_env. 
+        eapply set_eq_trans with (y:=r2); eauto.
+        eapply set_eq_trans with (y:=ids1 ++ [i1]); eauto.
+          apply set_eq_swap.          
+      simpl_env.
+      apply set_eq_app; auto using set_eq_refl.
+      apply set_eq_trans with (y:=(cmds_dominates_cmd (cs2' ++ [c']) 
+         (getCmdLoc c') ++ [i1]) ++ getArgsIDs la).
+        simpl_env.
+        apply set_eq_app; auto using set_eq_refl.
+          apply set_eq_swap.          
+
+        apply set_eq_app; auto using set_eq_refl.
+          apply set_eq_sym; auto.          
+
+    apply fold_left__opt_set_eq with (init2:=((getPhiNodesIDs ps2) ++ 
+      ((getCmdsIDs (cs2' ++ [c'])) ++ (getArgsIDs la)))) in Hinscope.
+      destruct Hinscope as [r3 [Hinscope Heq']].
+      exists r3.     
+      split; auto.
+      apply set_eq_app; auto using set_eq_refl.
+      apply set_eq_app; auto using set_eq_refl.
+      simpl_env in Hnotin.
+      apply set_eq_sym; auto.          
+Qed.
+
+Lemma cmds_dominates_cmd__cmds_dominates_cmd : forall cs2' c' c cs',
+  NoDup (getCmdsLocs (cs2'++[c']++[c]++cs')) ->
+  set_eq _ (cmds_dominates_cmd (cs2' ++ c' :: c :: cs') (getCmdLoc c))
+    (cmds_dominates_cmd (cs2' ++ c' :: c :: cs') (getCmdLoc c') ++
+     match getCmdID c' with
+     | Some id1 => [id1]
+     | None => nil
+     end).   
+Proof.
+  induction cs2'; intros c' c cs' Hnodup.
+    simpl in *.
+    inv Hnodup. simpl in H1.
+    remember (getCmdID c') as R.
+    destruct (eq_atom_dec (getCmdLoc c') (getCmdLoc c)).
+      contradict e; auto.
+
+      destruct (eq_atom_dec (getCmdLoc c) (getCmdLoc c)) as [_|n1];
+        try solve [contradict n1; auto].
+      destruct (eq_atom_dec (getCmdLoc c') (getCmdLoc c')) as [_|n2];
+        try solve [contradict n2; auto].
+      destruct R; auto using set_eq_refl.
+
+    simpl in *.
+    inv Hnodup.
+    rewrite getCmdsLocs_app in H1.
+    apply NotIn_inv in H1.    
+    destruct H1 as [H11 H12].
+    simpl in H12.
+    destruct (eq_atom_dec (getCmdLoc a) (getCmdLoc c)) as [e1 | ];
+      try solve [contradict e1; auto].
+    destruct (eq_atom_dec (getCmdLoc a) (getCmdLoc c')) as [e1 | ];
+      try solve [contradict e1; auto].
+    destruct (getCmdID a); auto.
+      apply IHcs2' in H2. clear IHcs2'.
+      simpl_env.
+       apply set_eq_app; auto using set_eq_refl.
+Qed.      
+
+Lemma inscope_of_cmd_cmd : forall f l2 ps2 cs2' c' c cs' tmn' ids1,
+NoDup (getCmdsLocs (cs2'++[c']++[c]++cs')) ->
+Some ids1 = inscope_of_cmd f (block_intro l2 ps2 (cs2'++[c']++[c]++cs') tmn') c' 
+  ->
+exists ids2, 
+  Some ids2 = 
+    inscope_of_cmd f (block_intro l2 ps2 (cs2'++[c']++[c]++cs') tmn') c /\
+  match getCmdID c' with
+  | Some id1 => set_eq _ (id1::ids1) ids2
+  | None => set_eq _ ids1 ids2
+  end.
+Proof.
+  intros f l2 ps2 cs2' c' c cs' tmn' ids1 Hnodup Hinscope.
+  unfold inscope_of_cmd in Hinscope.
+  unfold inscope_of_cmd.
+  destruct f as [[? ? ? la va] bs].
+  remember ((dom_analyze (fdef_intro (fheader_intro f t i0 la va) bs)) !! l2) as R.
+  destruct R as [R_contents R_bound].
+  apply cmds_dominates_cmd__cmds_dominates_cmd in Hnodup. simpl in *.
+  symmetry in Hinscope.
+  remember (getCmdID c') as R.
+  destruct R.
+    apply fold_left__opt_union with (init2:=[i1]) in Hinscope.
+    destruct Hinscope as [r2 [Hinscope Heq]].
+    apply fold_left__opt_set_eq with (init2:=((getPhiNodesIDs ps2) ++ 
+      ((cmds_dominates_cmd (cs2' ++ c' :: c :: cs') (getCmdLoc c)) ++
+      (getArgsIDs la)))) in Hinscope.
+      destruct Hinscope as [r3 [Hinscope Heq']].
+      exists r3.     
+      split; auto.
+        simpl_env. 
+        eapply set_eq_trans with (y:=r2); eauto.
+        eapply set_eq_trans with (y:=ids1 ++ [i1]); eauto.
+          apply set_eq_swap.          
+      simpl_env.
+      apply set_eq_app; auto using set_eq_refl.
+      apply set_eq_trans with (y:=(cmds_dominates_cmd (cs2' ++ [c']++[c]++cs') 
+         (getCmdLoc c') ++ [i1]) ++ getArgsIDs la).
+        simpl_env.
+        apply set_eq_app; auto using set_eq_refl.
+          apply set_eq_swap.          
+
+        apply set_eq_app; auto using set_eq_refl.
+          apply set_eq_sym; auto.          
+
+    apply fold_left__opt_set_eq with (init2:=((getPhiNodesIDs ps2) ++
+      ((cmds_dominates_cmd (cs2' ++ c' :: c :: cs') (getCmdLoc c)) ++
+      (getArgsIDs la)))) in Hinscope.
+      destruct Hinscope as [r3 [Hinscope Heq']].
+      exists r3.     
+      split; auto.
+      apply set_eq_app; auto using set_eq_refl.
+      apply set_eq_app; auto using set_eq_refl.
+      simpl_env in Hnodup.
+      apply set_eq_sym; auto.          
+Qed.
+
+Lemma inc__getLabel2Block_blocks : forall a bs 
+  (Hinc : incl [a] (bound_blocks bs)),
+  exists b : block, lookupAL block (genLabel2Block_blocks bs) a = Some b.
+Proof. 
+  intros.
+  induction bs; simpl in *; auto.
+    assert (J:=@Hinc a). simpl in J. destruct J; auto.
+    destruct a0; simpl in *.
+    destruct (a==l0); subst.
+      exists (block_intro l0 p c t). auto.
+
+      apply IHbs. intros x J.
+      assert (x=a) as EQ.
+        simpl in J. destruct J; auto. inversion H.
+      subst.      
+      apply Hinc in J. simpl in J.
+      destruct J as [J | J]; subst; auto.
+      contradict n; auto.
+Qed.
+
+Lemma fold_left__bound_blocks : forall ls0 fa t i0 la va bs l0 init,
+  incl ls0 (bound_blocks bs) ->
+  exists r, 
+    fold_left (inscope_of_block 
+      (fdef_intro (fheader_intro fa t i0 la va) bs) l0) ls0 (Some init) = 
+       Some r.
+Proof.
+  induction ls0; intros fa t i0 la va bs l0 init Hinc; simpl in *.
+    exists init. auto.
+
+    assert (incl ls0 (bound_blocks bs)) as J.
+      simpl_env in Hinc.
+      eapply incl_app_invr; eauto.
+    assert (exists b, lookupAL block (genLabel2Block_blocks bs) a = Some b) 
+      as Hlkup.
+      clear - Hinc.
+      simpl_env in Hinc.
+      apply incl_app_invl in Hinc.
+      apply inc__getLabel2Block_blocks; auto.
+
+    destruct Hlkup as [b Hlkup].
+    rewrite Hlkup. 
+    destruct (eq_atom_dec a l0); subst; auto.
+Qed.
+
+Lemma fold_left__spec : forall ls0 l0 init r f,
+  fold_left (inscope_of_block f l0) ls0 (Some init) = Some r ->
+    incl init r /\
+    (forall l1 b1, 
+      In l1 (ListSet.set_diff eq_atom_dec ls0 [l0]) -> 
+      lookupBlockViaLabelFromFdef f l1 = Some b1 ->
+      incl (getBlockIDs b1) r) /\
+    (forall id1,
+      In id1 r ->
+      In id1 init \/
+      exists b1, exists l1, In l1 (ListSet.set_diff eq_atom_dec ls0 [l0]) /\
+        lookupBlockViaLabelFromFdef f l1 = Some b1 /\
+        In id1 (getBlockIDs b1)
+    ).
+Proof.
+  induction ls0; intros l0 init r f Hfold; simpl in *.
+    inv Hfold.
+    split. apply incl_refl.
+    split; auto. 
+      intros ? ? Hfalse. inversion Hfalse.
+      
+    remember (lookupBlockViaLabelFromFdef f a) as R.
+    destruct R.
+      destruct (eq_atom_dec a l0); subst; auto.
+      apply IHls0 in Hfold.
+      destruct Hfold as [J1 [J2 J3]].
+      split.
+        eapply incl_app_invr; eauto.
+      split.
+        intros l1 b1 Hin Hlkup.
+        apply ListSet.set_add_elim in Hin.
+        destruct Hin as [Hin | Hin]; subst; eauto.                  
+          rewrite Hlkup in HeqR. inv HeqR.
+          eapply incl_app_invl; eauto.
+        intros id1 Hin.
+        apply J3 in Hin.
+        destruct Hin as [Hin | [b1 [l1 [H1 [H2 H3]]]]].
+          apply in_app_or in Hin.
+          destruct Hin as [Hin | Hin]; auto.
+          right. 
+          exists b. exists a.
+          split; auto.
+            apply ListSet.set_add_intro; auto.
+             
+          right.
+          exists b1. exists l1.
+          split; auto.
+            apply ListSet.set_add_intro; auto.
+
+      rewrite fold_left__none in Hfold. inversion Hfold.
+Qed.
+
+Inductive wf_phi_operands (f:fdef) (b:block) (id0:id) (t0:typ) : 
+    list_value_l -> Prop :=
+| wf_phi_operands_nil : wf_phi_operands f b id0 t0 Nil_list_value_l
+| wf_phi_operands_cons_vid : forall vid1 l1 vls b1 vb, 
+    vid1 <> id0 \/ (not (isReachableFromEntry f b)) ->
+    lookupBlockViaIDFromFdef f vid1 = Some vb ->
+    lookupBlockViaLabelFromFdef f l1 = Some b1 ->
+    blockDominates f vb b1 \/ (not (isReachableFromEntry f b)) ->
+    wf_phi_operands f b id0 t0 vls ->
+    wf_phi_operands f b id0 t0 (Cons_list_value_l (value_id vid1) l1 vls)
+| wf_phi_operands_cons_vc : forall c1 l1 vls, 
+    wf_phi_operands f b id0 t0 vls ->
+    wf_phi_operands f b id0 t0 (Cons_list_value_l (value_const c1) l1 vls).
+
+Definition check_list_value_l (f:fdef) (b:block) (vls:list_value_l) := 
+  let ud := genBlockUseDef_fdef f in
+  let vls1 := unmake_list_value_l vls in
+  let '(vs1,ls1) := List.split vls1 in 
+  let ls2 := predOfBlock b ud in
+  (length ls2 > 0)%nat /\
+  AtomSet.set_eq _ ls1 ls2 /\
+  NoDup ls1.
+
+Definition wf_phinode (f:fdef) (b:block) (p:phinode) :=
+let '(insn_phi id0 t0 vls0) := p in
+wf_phi_operands f b id0 t0 vls0 /\ check_list_value_l f b vls0. 
+
 (*****************************)
 (*
 *** Local Variables: ***
