src/ssa/vellvm.v
@@ -1,0 +1,25 @@
+Add LoadPath "../ssa/ott".
+Add LoadPath "../ssa/monads".
+Add LoadPath "../ssa".
+Add LoadPath "../ssa/compcert".
+Add LoadPath "../../../theory/metatheory_8.3".
+Add LoadPath "../TV".
+Require Import ssa_def.
+Require Import ssa_lib.
+Require Import ssa_static.
+Require Import genericvalues.
+Require Import targetdata.
+
+Export LLVMsyntax.
+Export LLVMlib.
+Export LLVMgv.
+Export LLVMtd.
+Export LLVMwf.
+
+(*****************************)
+(*
+*** Local Variables: ***
+*** coq-prog-name: "coqtop" ***
+*** coq-prog-args: ("-emacs-U" "-I" "~/SVN/sol/vol/src/ssa/monads" "-I" "~/SVN/sol/vol/src/ssa/ott" "-I" "~/SVN/sol/vol/src/ssa/compcert" "-I" "~/SVN/sol/theory/metatheory_8.3" "-I" "~/SVN/sol/vol/src/TV") ***
+*** End: ***
+ *)
